spec/design/TCB_H.thy
@@ -36,7 +36,6 @@ requalify_consts
   msgRegisters
   tpidrurwRegister
   fromVPtr
-  asUser
 end
 
 defs decodeTCBInvocation_def:
@@ -588,5 +587,13 @@ defs threadSet_def:
         setObject tptr $ f tcb
 od)"
 
+
+defs asUser_def:
+"asUser tptr f\<equiv> (do
+        uc \<leftarrow> threadGet  (atcbContextGet o tcbArch) tptr;
+        (a, uc') \<leftarrow> select_f (f uc);
+        threadSet (\<lambda> tcb. tcb \<lparr> tcbArch := atcbContextSet uc' (tcbArch tcb)\<rparr>) tptr;
+        return a
+od)"
 
 end
