spec/design/skel/ARM/ArchTCB_H.thy
@@ -16,7 +16,7 @@ context Arch begin global_naming ARM_H
 #INCLUDE_HASKELL SEL4/Object/TCB/ARM.lhs CONTEXT ARM_H
 
 
-#INCLUDE_HASKELL SEL4/Object/TCB.lhs Arch= ONLY archThreadGet archThreadSet asUser
+#INCLUDE_HASKELL SEL4/Object/TCB.lhs Arch= ONLY archThreadGet archThreadSet
 
 end
 end
