spec/design/skel/Structures_H.thy
@@ -40,6 +40,8 @@ requalify_consts
   newArchTCB
   fromPPtr
   PPtr
+  atcbContextGet
+  atcbContextSet
 
 end
 
