spec/machine/ARM/MachineTypes.thy
@@ -369,5 +369,8 @@ end
 
 (*>*)
 end_qualify
+context Arch begin global_naming ARM
 
+
+end
 end
